Semantic/Prelude.lean
@@ -1,9 +1,9 @@
-class HasDenotation (T : Type) (Env : Type) (Denot : outParam Type) where
-  interp : Env -> T -> Denot
+class HasDenotation (T : Type) (Env : Type) (TEnv : Type) (Denot : outParam Type) where
+  interp : Env -> TEnv -> T -> Denot
 
-notation:max "⟦" T "⟧_[" ρ "]" => HasDenotation.interp ρ T
+notation:max "⟦" T "⟧_[" ρ "," φ "]" => HasDenotation.interp ρ φ T
 
-class HasExpDenotation (T : Type) (Env : Type) (Denot : outParam Type) where
-  interp : Env -> T -> Denot
+class HasExpDenotation (T : Type) (Env : Type) (TEnv : Type) (Denot : outParam Type) where
+  interp : Env -> TEnv -> T -> Denot
 
-notation:max "⟦" T "⟧e_[" ρ "]" => HasExpDenotation.interp ρ T
+notation:max "⟦" T "⟧e_[" ρ "," φ "]" => HasExpDenotation.interp ρ φ T
